theories/Dot/lr/path_wp.v
@@ -1,5 +1,5 @@
 From iris.proofmode Require Import tactics.
-From D Require Import iris_prelude.
+From D Require Import iris_prelude iris_extra.det_reduction.
 From D.Dot Require Import dlang_inst rules lr_syn_aux syn.path_repl.
 From D.pure_program_logic Require Import lifting.
 
