theories/Dot/misc_unused/skeleton_termination.v
@@ -1,5 +1,6 @@
 From iris.program_logic Require Import
      ectx_lifting ectx_language ectxi_language.
+From D Require Import iris_extra.det_reduction.
 From D.Dot Require Import syn traversals skeleton.
 From D.Dot Require rules.
 
@@ -26,22 +27,6 @@ Notation same_skeleton_path := (forall_traversal_path same_skeleton_trav ()).
 Notation same_skeleton_ty := (forall_traversal_ty same_skeleton_trav ()).
 End AlternativeDef.
 
-Section prim_step_det.
-Import rules.
-Lemma prim_step_pure e1 e2 σ1 κ σ2 efs :
-  prim_step e1 σ1 κ e2 σ2 efs → PureExec True 1 e1 e2.
-Proof. inversion 1; simplify_eq/=. by eapply pure_exec_fill, head_step_pure. Qed.
-
-Lemma prim_step_det e e1 e2 σ1 κ σ2 efs :
-  prim_step e σ1 κ e1 σ2 efs →
-  prim_step e σ1 κ e2 σ2 efs → e1 = e2.
-Proof.
-  move => /prim_step_pure /(_ I) /(nsteps_once_inv _ _) [_ /(_ ()) Hdet]
-    Hstep; destruct σ1, σ2.
-  by edestruct Hdet => //; destruct_and!; simplify_eq/=.
-Qed.
-End prim_step_det.
-
 Lemma pure_step_prim (t1 t1' : tm) :
   pure_step t1 t1' →
   reducible_no_obs t1 () ∧ prim_step t1 () [] t1' () [].
@@ -55,27 +40,15 @@ Qed.
 Theorem simulation_skeleton_pure_step {t1 t1' t2 : tm} :
   same_skel_tm t1 t2 →
   pure_step t1 t1' → ∃ t2', pure_step t2 t2' ∧ same_skel_tm t1' t2'.
-Proof.
-  move => Hskel /pure_step_prim [Hred Hstep].
-  pose proof simulation_skeleton as (t2' & ? & ?) => //.
-  exists t2'; int.
-  have Hred' := (same_skel_reducible_no_obs Hskel Hred).
-  constructor; intros [] *; cbn; first done; destruct σ2.
-  intros Hstep'; prim_step_inversion Hstep'.
-  int; exact: prim_step_det.
-Qed.
+Proof. setoid_rewrite <-prim_step_pure_eq'; exact: simulation_skeleton. Qed.
 
 Theorem simulation_skeleton_pure_steps {t_s t_r u_s : tm} :
   same_skel_tm t_s u_s →
   rtc pure_step t_s t_r →
   ∃ u_r, rtc pure_step u_s u_r ∧ same_skel_tm t_r u_r.
 Proof.
-  move => /= Hst Hsteps; move: u_s Hst.
-  dependent induction Hsteps; intros; first by exists u_s; eauto.
-  rename H into Hstep, x into t_s, y into t', z into t_r.
-  have [/= u' [? Hst']] := simulation_skeleton_pure_step Hst Hstep.
-  pose proof (IHHsteps _ Hst') as (u_r&?&?).
-  exists u_r; split_and!; by [|exact: rtc_l].
+  setoid_rewrite pure_steps_erased'; intros.
+  by eapply simulation_skeleton_erased_steps, elem_of_list_singleton.
 Qed.
 
 Lemma terminates_same_skel {e e_s}:
